src/proof/kubernetes_model/delete.v
@@ -243,7 +243,7 @@ Proof.
     destruct H as (_ & _ & _ & Hvalid_kmeta).
     unfold ObjectMetaV.valid in Hvalid_kmeta.
     destruct Hvalid_kmeta as
-      (_ & _ & _ & _ & _ & _ & _ & _ & Hvalid_finalizers & _).
+      (_ & _ & _ & _ & _ & _ & _ & _ & _ & Hvalid_finalizers & _).
     iPoseProof (kview.own_meta_exists2 with "Hinv_Hown_abs Hown_meta_frag") as "%H". 1: done.
     destruct H as (Hkmeta_eq & _).
     rewrite <- Hkmeta_eq in Hvalid_finalizers.
